added concrete functions to HelperFuns.ec, got rid of some smts and cleaned uo some code

HelperFuns.ec
@@ -1,43 +1,334 @@
-require import SmtMap List Finite FSet.
+pragma Goals:printall. 
+require import SmtMap List Finite FSet CoreMap Int AllCore.
 
+op eq_except_l ['a] (P : 'a -> bool) (m1 m2 : 'a list) : bool =
+  forall x, !P x => (x \in m1) <=> (x \in m2).
+
+op sbset ['a 'b]  (m1 m2 : ('a, 'b) fmap) : bool
+ = eq_except (fun x => !(x \in m1)) m1 m2.
 
 lemma wtp ['a] : forall (l : 'a list),  uniq l => size l = card (oflist l). 
 proof. elim. smt. progress. smt.
 qed.
 
-op eq_except_l ['a] (P : 'a -> bool) (m1 m2 : 'a list) : bool =
-  forall x, !P x => (x \in m1) <=> (x \in m2).
-
 lemma eel1 (P : 'a -> bool) m1 m2 x : eq_except_l P m1 m2 => eq_except_l P (x :: m1) (x :: m2).
 smt.
 qed.
-
 
 lemma thm5 ['a 'b]  (m : ('a, 'b) fmap) x : x \in m => exists y, m.[x] = Some y.
 smt.
 qed.
 
-op sbset ['a 'b]  (m1 m2 : ('a, 'b) fmap) : bool
- = eq_except (fun x => !(x \in m1)) m1 m2.
+(* function that checks if fmap does not have duplicates: true = does not have duplicates *)
+op up (m : ('a, 'b) fmap) : 'a -> 'b -> bool = (fun (x :'a) (y :'b) => !rng (rem m x) y).
+op uniqf ['a 'b]  (m : ('a, 'b) fmap) : bool = filter (up m) m = m.
 
- 
-(* delcarative specification of a hasdup function *)
-op hasdup ['a 'b] : ('a, 'b) fmap -> bool.
-axiom thm3 ['a 'b] m (c : 'b) (x y : 'a) : !hasdup m => m.[x] = Some c => m.[y] = Some c => x = y.
-axiom thm4 (m1 m2 : ('a, 'b) fmap) : !hasdup m2 => sbset m1 m2  => !hasdup m1.
-axiom thm11 (m : ('a, 'b) fmap) x c : !hasdup m => x \notin m => hasdup m.[x <- c] = mem (to_seq (rng m)) c .
-axiom thm6 (m : ('a, 'b) fmap) c c' y : m.[c] = Some y => m.[c'] = Some y => c <> c' => hasdup m.
-axiom hde : hasdup (empty<: 'a, 'b>) = false.
- 
-(* declarative specification of a domain searching function *)
-op solve ['a 'b]  (m : ('a, 'b) fmap) (x : 'b) : 'a list.
-axiom thm1 ['a 'b] (x : 'a) m (y : 'b) : !hasdup m => m.[x] = Some y => solve m y = [x].
+abbrev (\inp) ['a, 'b] (x : 'a * 'b) (m : ('a, 'b) fmap) : bool = dom m x.`1 /\ m.[x.`1] = Some x.`2.
 
-(* declarative specification of a range searching function *)
-op lookupc : ('a, 'b) fmap -> 'b -> bool.
-axiom thm2 (m : ('a,'b) fmap) c : lookupc m c = true => exists x, m.[x] = Some c.
-axiom thm7 (m : ('a, 'b) fmap) x c  c' : lookupc m  c = false => c <> c' => lookupc m.[x <- c']  c = false.
-axiom thm9 (m : ('a, 'b) fmap) x c : lookupc m.[x <- c]  c = true.
-axiom thm10 (m : ('a, 'b) fmap) x : x \in m => lookupc m (oget m.[x]) = true.
+
+lemma filterLemma1 (P : ('a -> 'b -> bool)) (m : ('a, 'b) fmap): 
+  filter P m = m => (forall x y, m.[x] = Some y => P x y).
+proof.
+progress. 
+smt.  
+qed.
+
+
+lemma filterLemma1' (P : ('a -> 'b -> bool)): forall (m : ('a, 'b) fmap),
+  (forall x y, m.[x] = Some y => P x y) => filter P m = m.
+proof. 
+apply fmapW. progress. 
+rewrite -fmap_eqP. progress. smt.
+progress.
+smt.
+qed.
+
+
+lemma fL (P : ('a -> 'b -> bool)) (m : ('a, 'b) fmap): 
+  filter P m = m <=> (forall x y, m.[x] = Some y => P x y).
+proof.
+smt(filterLemma1 filterLemma1').
+qed.
+
+
+lemma filterLemma2 (m : ('a, 'b) fmap) (P : ('a -> 'b -> bool)): 
+  filter P m <> m => (exists x y, m.[x] = Some y => P x y = false).
+proof.
+progress.
+smt. 
+qed.
+
+
+lemma fL2 (m : ('a, 'b) fmap): 
+(forall x y, m.[x] = Some y => up m x y) <=>
+      uniqf m.
+proof.
+split. progress.
+apply filterLemma1' in H.
+rewrite /uniqf. 
+smt.
+smt.
+qed.
+
+
+lemma uniqfL2 (m : ('a, 'b) fmap): 
+   !uniqf m <=> (exists x y, x <> y /\ m.[x] = m.[y] /\ m.[x] <> None).
+proof.
+split. progress.
+rewrite /uniqf/up in H. smt.
+progress.
+rewrite -domE in H1.  
+case(y \notin m). smt.
+simplify. move => H2.
+rewrite /uniqf/up/rng. 
+have ->: (filter (fun (x0 : 'a) (y0 : 'b) => ! (exists (x1 : 'a), (rem m x0).[x1] = Some y0)) m <> m) = (filter (fun (x0 : 'a) (y0 : 'b) => (forall (x1 : 'a), (rem m x0).[x1] <> Some y0)) m <> m).
+smt.
+have : exists b, m.[x] = Some b. smt.
+move => H3.
+smt. 
+qed.
+
+
+lemma uniqfL1 (m : ('a, 'b) fmap): 
+   (forall x y, x \in m => y \in m => x <> y => m.[x] <> m.[y]) <=> uniqf m.
+proof.
+split. progress.
+rewrite /uniqf/up.
+smt.
+smt.
+qed.
+
+
+lemma helper (m : ('a, 'b) fmap) (x : 'a) (y : 'b): 
+   (x, y) \inp (rem m x) => (x, y) \inp m.
+proof.
+progress.
+smt. smt.
+qed.
+
+
+lemma uniqf_rem (m : ('a, 'b) fmap) (x : 'a): 
+   uniqf m => uniqf (rem m x).
+proof.
+progress.
+smt.
+qed.
+
+
+lemma l21 (m : ('a, 'b) fmap): 
+(forall x y, m.[x] = Some y => up m x y) =>
+      (forall (x : 'a), uniqf (rem m x)).
+proof.
+progress.
+rewrite fL2 in H.
+smt. 
+qed.
+
+
+lemma mainl1 : uniqf (empty<: 'a, 'b>) = true.
+proof.
+rewrite /uniqf.
+have ->: (filter (fun (x : 'a) (y : 'b) => ! rng (rem empty x) y) empty) = empty. 
+smt.
+auto.
+qed.
+
+
+lemma mainl2 (m : ('a, 'b) fmap): 
+(forall (x: 'a) (y : 'b), uniqf m.[x <- y]) => 
+   (forall (x: 'a) (y: 'b), (uniqf (rem m x) /\ !rng (rem m x) y)).
+proof.
+progress. 
+have : x \in  m.[x <- y].
+smt. progress.
+have : uniqf m.[x<-y]. smt. 
+progress. 
+smt.
+have : uniqf m.[x<-y]. smt. 
+progress.
+smt.
+qed.
+
+
+(* function that checks if fmap has duplicates: true = has duplicates *)
+op hasdup (m : ('a, 'b) fmap): bool = !uniqf m.
+
+lemma hde : hasdup (empty<: 'a, 'b>) = false.
+proof. 
+rewrite /hasdup/uniqf. 
+smt.
+qed.
+
+lemma thm3 ['a 'b] m (c : 'b) (x y : 'a) : !hasdup m => m.[x] = Some c => m.[y] = Some c => x = y.
+proof.
+rewrite /hasdup.
+progress.
+rewrite -uniqfL1 in H.
+smt. 
+qed.
+
+lemma thm4 (m1 m2 : ('a, 'b) fmap) : !hasdup m2 => sbset m1 m2  => !hasdup m1.
+proof.
+rewrite /hasdup.
+progress.
+smt. 
+qed.
+
+lemma thm11 (m : ('a, 'b) fmap) x c : !hasdup m => x \notin m => hasdup m.[x <- c] = mem (to_seq (rng m)) c.
+proof.
+progress.
+rewrite mem_to_seq.
+rewrite finite_rng.
+smt. 
+qed.
+
+lemma thm6 (m : ('a, 'b) fmap) c c' y : m.[c] = Some y => m.[c'] = Some y => c <> c' => hasdup m.
+proof.
+progress.
+smt. 
+qed.
+
+
+(* domain searching function *)
+op solve ['a 'b]  (m : ('a, 'b) fmap) (y : 'b) : 'a list = to_seq (dom (filter (fun (x : 'a) (y' : 'b) => y' = y) m)). 
+
+(* completeness *)
+lemma solve1 ['a 'b] (x : 'a) (m : ('a, 'b) fmap) (y : 'b) : m.[x] = Some y => x \in solve m y.
+proof.
+progress.
+rewrite /solve.
+case(!dom (filter (fun (_ : 'a) (y' : 'b) => y' = y) m) x). smt.
+simplify. progress.
+smt.
+qed.
+
+
+(* soundness *)
+lemma solve2 ['a 'b] (x : 'a) (m : ('a, 'b) fmap) (y : 'b) : x \in solve m y => m.[x] = Some y.
+proof.
+progress.
+rewrite /solve in H.
+have : (x, y) \inp (filter (fun (_ : 'a) (y' : 'b) => y' = y) m). smt. 
+move => H1.
+smt. 
+qed.
+
+
+lemma thm1 ['a 'b] (x : 'a) m (y : 'b) : !hasdup m => m.[x] = Some y => x \in solve m y => solve m y = [x].
+proof.
+progress. 
+rewrite /hasdup in H. 
+rewrite -uniqfL1 in H.
+case(x \notin m). smt. simplify. move => H2.
+case(m = empty). smt. move => H3.
+
+have : is_finite (dom (filter (fun (_ : 'a) (y' : 'b) => y' = y) m)). 
+apply finite_dom. move => h.
+have : uniq (to_seq (dom (filter (fun (_ : 'a) (y' : 'b) => y' = y) m))). smt. move => h1.
+pose xs := to_seq (dom (filter (fun (_ : 'a) (y' : 'b) => y' = y) m)).
+
+case(xs = []). move => H4.
+apply solve1 in H0. rewrite /solve in H0.
+smt. move => H4.
+
+case(exists z, xs = [z]).
+progress.
+case(z=x). progress.
+move => H6. 
+rewrite /solve in H1.  smt. 
+rewrite negb_exists. progress.
+
+case(exists z z1 (zs : 'a list), xs = [z;z1] ++ zs).
+progress. 
+case(zs = []). move => h2. 
+case(z=x). progress. 
+have : z1 \in solve m y. rewrite /solve. smt. move => hh.
+apply solve2 in hh. smt. move => H7.
+have : z \in solve m y. rewrite /solve. smt. move => hh.
+apply solve2 in hh. smt. move => H7.
+case(z=x). progress. 
+have : z1 \in solve m y. rewrite /solve. smt. move => hh.
+apply solve2 in hh. smt. move => H8. 
+have : z \in xs. smt. move => H9.
+apply solve2 in H9. smt.
+rewrite negb_exists. 
+have ->: (forall (a : 'a), ! (fun (a0 : 'a) => exists (z1 : 'a) (zs : 'a list), xs = a0 :: z1 :: zs) a) = (forall (a : 'a), (fun (a0 : 'a) => forall (z1 : 'a) (zs : 'a list), xs <> a0 :: z1 :: zs) a). smt. progress.
+rewrite /solve. have : uniqf m. smt. progress.
+rewrite /solve in H1.
+have ->: (to_seq (dom (filter (fun (_ : 'a) (y' : 'b) => y' = y) m)) = [x]) = (xs = [x]). smt. 
+
+case(rem x xs = []). smt. progress. 
+case(exists x1, x1 \in rem x xs).  
+progress.
+case(x1=x). smt. progress.
+case(x1 \in xs). progress. 
+
+have : dom (filter (fun (_ : 'a) (y' : 'b) => y' = y) m) x1. smt. progress.
+case(x1 \in solve m y). smt. progress.
+have : m.[x1] <> Some y. smt. progress.  
+have : x1 \in to_seq (dom (filter (fun (_ : 'a) (y' : 'b) => y' = y) m)).
+  smt. progress. apply solve2 in H15. smt. 
+progress. smt. 
+rewrite negb_exists. simplify. progress.  
+case((rem x xs) = []). smt. progress.
+apply mem_eq0 in H9. smt. 
+qed.
+
+
+(* range searching function *)
+op lookupc (m : ('a, 'b) fmap) (y : 'b) : bool = (solve m y) <> [].
+
+lemma thm2 (m : ('a,'b) fmap) y : lookupc m y => exists x, m.[x] = Some y.
+proof. 
+progress. 
+rewrite /lookupc/solve in H.
+pose xs := to_seq (dom (filter (fun (_ : 'a) (y' : 'b) => y' = y) m)).
+have : xs <> []. smt. progress.  
+case(exists x, x \in xs). progress. exists x. apply solve2 in H1. 
+auto.  
+rewrite negb_exists. simplify. progress. 
+apply mem_eq0 in H1. smt. 
+qed.
+
+
+lemma thm7 (m : ('a, 'b) fmap) x c c' : !lookupc m c => c <> c' => !lookupc m.[x <- c'] c.
+proof.
+progress. 
+rewrite /lookupc/solve in H.
+have : to_seq (dom (filter (fun (_ : 'a) (y' : 'b) => y' = c) m)) = [].
+smt. progress.
+have : (filter (fun (x : 'a) (y' : 'b) => y' = c) m) = empty. smt. move => H2.
+rewrite /lookupc/solve =>//=. 
+case(x \notin m). smt. progress.
+case(m.[x] = Some c'). smt. move => H4.
+case(m.[x] = Some c). smt. move => H5.
+smt. 
+qed.
+
+
+lemma thm9 (m : ('a, 'b) fmap) x c : lookupc m.[x <- c] c.
+proof.
+rewrite /lookupc/solve.
+have : x \in to_seq (dom (filter (fun (_ : 'a) (y' : 'b) => y' = c) m.[x <- c])).
+smt.  
+progress. smt.
+qed.
+
+lemma thm10 (m : ('a, 'b) fmap) x : x \in m => lookupc m (oget m.[x]).
+proof.
+progress. 
+pose c := oget m.[x].
+rewrite /lookupc.
+case(m = empty). smt. move => h.
+case(x \in (filter (fun (_ : 'a) (y' : 'b) => y' = c) m)).  
+smt. 
+smt. 
+qed.
+
+
+
+
+
+
 
 
