ConstComm.ec
@@ -47,19 +47,19 @@ declare module A : AdvSNM.
 
 lemma lll &m : 
  Pr[ C_SEG0(ConstComm,A).main(ler,md) @ &m : res ] = 0%r.
-byphoare. hoare. proc.
+byphoare =>//. hoare. proc.
 inline*. wp.  
 conseq (_: _ ==> true).
 call (_:true). call (_:true). wp. rnd. wp.
 skip. auto.
-auto. auto.
 qed.
 
 
 (* ConstComm satisfies the non-malleability by Crescenzo et al. *)
 lemma cresc_const_comm &m : forall (S <: Simulator),  Pr[ C_SEG0(ConstComm,A).main(ler,md) @ &m : res ]
  - Pr[ C_SEG1(ConstComm,S).main(ler,md) @ &m : res ] <= 0%r.
-proof. move => S. rewrite lll. smt. qed.
+proof. move => S. rewrite lll. smt. 
+qed.
 
 end section.
 end CrescenzoSNM.
@@ -114,13 +114,13 @@ op myrel = fun (m1 m2 : message) => m1 <> m2.
 op myd = duniform [false;true].
 
 lemma qq &m : Pr[ A_SEG0(AritaA).main(myrel,myd) @ &m : res ] = 1%r.
-proof. byphoare (_: arg = (myrel, myd) ==> _). proc.
+proof. byphoare (_: arg = (myrel, myd) ==> _) =>//. proc.
 inline*. rewrite /Ver. wp.  simplify.
 seq 3 : (rel = myrel /\ md = myd).
 rnd. rnd. rnd. skip. auto. rnd.  rnd.  rnd.  skip.  progress. smt. smt. smt. skip .  progress.
 smt.
 smt. hoare. simplify.
-rnd. rnd. rnd. skip. auto. auto. auto. auto.
+rnd. rnd. rnd. skip. auto. auto. 
 qed.
 
 section.
@@ -131,7 +131,7 @@ axiom S_ll : islossless S.simulate.
 
 
 lemma pp &m : Pr[ A_SEG1(S).main(myrel,myd) @ &m : res ] = 1%r/2%r.
-proof. byphoare (_: arg = (myrel, myd) ==> _). proc.
+proof. byphoare (_: arg = (myrel, myd) ==> _) =>//. proc.
 swap 2 1.
 seq 2 :  true 1%r (1%r/2%r)   (1%r/2%r) 0%r (rel = myrel /\ md = myd) .
 call (_:true). rnd. skip.  auto.
@@ -143,7 +143,7 @@ have ->: (fun (x : message) => x <> m'{hr} /\ x <> m'{hr})
 apply fun_ext. smt.
 rewrite /myd.
 rewrite duniformE. smt.
-exfalso. auto. auto. auto. auto.
+exfalso. auto. auto. 
 qed.
 
 
