WholeMsg.ec
@@ -41,12 +41,12 @@ local module W' = {
 local lemma scx1 &m x:
     Pr[ W'.main(x) @ &m : res /\ W'.m = m1 ]
   = 1%r/2%r * Pr[ T.main(m1,x) @ &m : res ].
-proof. byphoare (_: (glob T) = (glob T){m} /\ a = x ==> _). 
+proof. byphoare (_: (glob T) = (glob T){m} /\ a = x ==> _) => //. 
 proc. 
 pose z := (Pr[ T.main(m1,x) @ &m : res ]).
 seq 1 : (W'.m = m1) (1%r/2%r)  z (1%r/2%r) 0%r  ((glob T) = (glob T){m} /\ a = x).
 rnd.  skip. progress. 
-rnd.  skip. progress. rewrite duniformE. progress. 
+rnd.  skip. progress. rewrite duniformE =>//=. 
 have : m1 <> m2. apply m1_and_m2_diff. progress.
 case(m1 = m2) => //. progress. rewrite eq_sym in H0. rewrite H0. smt. 
 have phr : phoare[ T.main : (glob T) = (glob T){m} /\ arg = (m1, x) ==> res ] = Pr[ T.main(m1,x) @ &m : res ].
@@ -54,20 +54,20 @@ bypr. progress. byequiv.
 proc*. call (_:true). skip.
 progress. auto. smt. smt. auto. auto.
 call phr. skip. progress.
-hoare. call (_:true). skip. progress. rewrite H. trivial.
-rewrite /z.  auto. auto. auto. 
+hoare. call (_:true). skip. progress. rewrite H =>//=. 
+rewrite /z =>//.   
 qed.
 
 
 local lemma scx2 &m x:
     Pr[ W'.main(x) @ &m : res /\ W'.m = m2 ]
   = 1%r/2%r * Pr[ T.main(m2,x) @ &m : res ].
-proof. byphoare (_: (glob T) = (glob T){m} /\ a = x ==> _). 
+proof. byphoare (_: (glob T) = (glob T){m} /\ a = x ==> _) =>//. 
 proc. 
 pose z := (Pr[ T.main(m2,x) @ &m : res ]).
 seq 1 : (W'.m = m2) (1%r/2%r)  z (1%r/2%r) 0%r  ((glob T) = (glob T){m} /\ a = x).
 rnd.  skip. auto. 
-rnd.  skip. progress. rewrite duniformE. progress. 
+rnd.  skip. progress. rewrite duniformE =>//=.  
 have : m1 <> m2. apply m1_and_m2_diff. progress.
 case(m1 = m2) => //. progress. rewrite H0. smt. 
 have phr : phoare[ T.main : (glob T) = (glob T){m} /\ arg = (m2, x) ==> res ] = Pr[ T.main(m2,x) @ &m : res ].
@@ -75,8 +75,8 @@ bypr. progress. byequiv.
 proc*. call (_:true). skip.
 progress. smt. smt. auto. auto.
 call phr. skip. progress.
-hoare. call (_:true). skip. progress. rewrite H. trivial.
-rewrite /z.  auto. auto. auto. 
+hoare. call (_:true). skip. progress. rewrite H =>//. 
+rewrite /z =>//.   
 qed.
 
 
@@ -96,7 +96,7 @@ rewrite supp_duniform mem_seq2 in H.
 elim H => [mL1 | mL2] => //.   
 have : m1 <> m2. apply m1_and_m2_diff. progress. rewrite eq_sym in H2. apply H2.
 reflexivity.
-rewrite scx1 scx2. progress. 
+rewrite scx1 scx2 =>//.  
 qed.
 
    
